src/SubstSemantics.v
@@ -32,6 +32,16 @@ match clock with
          | EVar n => Fail
          | EFunId n => Fail
          | EFun vl e => Res (EFun vl e)
+         | ENil => Res (ENil)
+         | ECons e1 e2 => match eval n e2 with
+                          | Res v2 => match eval n e1 with
+                                     | Res v1 => Res (ECons v1 v2)
+                                     | Fail => Fail
+                                     | Timeout => Timeout
+                                     end
+                          | Fail => Fail
+                          | Timeout => Timeout
+                          end
          | EApp exp l => match eval n exp with
                          (** In Core Erlang this check only happens later *)
                          | Res (EFun vl e) =>
@@ -94,12 +104,12 @@ Proof.
     - simpl. apply IHel. exact Heqr0. simpl in H0. lia.
 Qed.
 
-Theorem list_result_is_value l : forall clock vals,
-  (forall e v : Exp, eval clock e = Res v -> is_value v)
+Theorem list_result_VALCLOSED l : forall clock vals,
+  (forall e v : Exp, eval clock e = Res v -> VALCLOSED v)
 ->
   eval_list (eval clock) l = Res vals
   ->
-  forall i, i < length vals -> is_value (nth i vals (ELit 0)).
+  forall i, i < length vals -> VALCLOSED (nth i vals (ELit 0)).
 Proof.
   induction l; intros.
   * simpl in H0. inversion H0. subst. inversion H1.
@@ -107,27 +117,7 @@ Proof.
     break_match_hyp; try congruence. inversion H0. subst.
     pose (IHl _ _ H Heqr0). destruct i.
     - simpl. auto.
-    - apply i0. simpl in H1. lia.
-Qed.
-
-Theorem result_is_value :
-  forall clock e v, eval clock e = Res v -> is_value v.
-Proof.
-  intro. induction clock; intros.
-  * inversion H.
-  * destruct e; inversion H.
-    - constructor.
-    - constructor.
-    - break_match_hyp; inversion H1. break_match_hyp; try congruence.
-      + break_match_hyp; try congruence. break_match_hyp. 2: congruence. apply IHclock in H1. auto.
-    - break_match_hyp; try congruence. apply IHclock in H1. auto.
-    - apply IHclock in H1. auto.
-    - break_match_hyp; try congruence. break_match_hyp; try congruence; break_match_hyp; try congruence.
-      break_match_hyp; try congruence.
-      + inversion H1. constructor.
-    - break_match_hyp; try congruence. break_match_hyp; try congruence.
-      destruct l; apply IHclock in H1; auto.
-      all: apply IHclock in H1; auto.
+    - apply v1. simpl in H1. lia.
 Qed.
 
 Lemma foo x :
@@ -157,28 +147,28 @@ Definition terminating (e : Exp) : Prop :=
 Reserved Notation "⟨ fs , e ⟩ --> ⟨ fs' , e' ⟩" (at level 50).
 Inductive step : FrameStack -> Exp -> FrameStack -> Exp -> Prop :=
 (**  Reduction rules *)
-| red_app_start v hd tl xs (H : is_value v):
+| red_app_start v hd tl xs (H : VALCLOSED v):
   ⟨ (FApp1 (hd::tl))::xs, v ⟩ --> ⟨ (FApp2 v tl [])::xs, hd⟩
 
 | red_app_fin xs e :
   ⟨ (FApp1 [])::xs, EFun [] e ⟩ --> ⟨ xs, e.[EFun [] e/] ⟩
 
-| app2_step v (H : is_value v) hd tl vs (H2 : Forall is_value vs) xs v' (H' : is_value v') :
+| app2_step v (H : VALCLOSED v) hd tl vs (H2 : Forall (fun v => VALCLOSED v) vs) xs v' (H' : VALCLOSED v') :
   ⟨ (FApp2 v (hd::tl) vs) :: xs, v' ⟩ --> ⟨ (FApp2 v tl (vs ++ [v'])) :: xs, hd ⟩
 
-| red_app2 vl e vs v xs (H2 : Forall is_value vs) : 
-  is_value v -> length vl = S (length vs) ->
+| red_app2 vl e vs v xs (H2 : Forall (fun v => VALCLOSED v) vs) : 
+  VALCLOSED v -> length vl = S (length vs) ->
   ⟨ (FApp2 (EFun vl e) [] vs) :: xs, v ⟩ --> ⟨ xs,  e.[list_subst (EFun vl e :: (vs ++ [v])) idsubst] ⟩
 
-| red_let val e2 xs v (H : is_value val) : ⟨ (FLet v e2)::xs, val ⟩ --> ⟨ xs, e2.[val/] ⟩
+| red_let val e2 xs v (H : VALCLOSED val) : ⟨ (FLet v e2)::xs, val ⟩ --> ⟨ xs, e2.[val/] ⟩
 
 | red_if_true e2 e3 xs : ⟨ (FIf e2 e3)::xs, ELit 0 ⟩ --> ⟨ xs, e2 ⟩
 
-| red_if_false e2 e3 v xs (H : is_value v) :
+| red_if_false e2 e3 v xs (H : VALCLOSED v) :
   v <> ELit 0 ->
   ⟨ (FIf e2 e3)::xs, v ⟩ --> ⟨ xs, e3 ⟩
 
-| red_plus_left e2 xs v (H : is_value v): ⟨ (FPlus1 e2)::xs, v ⟩ --> ⟨ (FPlus2 v (* H *))::xs, e2 ⟩
+| red_plus_left e2 xs v (H : VALCLOSED v): ⟨ (FPlus1 e2)::xs, v ⟩ --> ⟨ (FPlus2 v (* H *))::xs, e2 ⟩
 
 | red_plus_right xs n m :
    ⟨ (FPlus2 (ELit n) (* P *))::xs, (ELit m) ⟩ --> ⟨ xs, ELit (n + m) ⟩ 
@@ -186,11 +176,20 @@ Inductive step : FrameStack -> Exp -> FrameStack -> Exp -> Prop :=
 | red_letrec xs f vl b e:
   ⟨ xs, ELetRec f vl b e ⟩ --> ⟨ xs, e.[EFun vl b/] ⟩
 
+| red_cons1 xs v2 e1 (H : VALCLOSED v2):
+  ⟨ FCons1 e1::xs, v2⟩ --> ⟨FCons2 v2::xs, e1 ⟩
+
+| red_cons2 xs v2 v1 (H : VALCLOSED v1) (H0 : VALCLOSED v2):
+  ⟨ FCons2 v2::xs, v1⟩ --> ⟨xs, ECons v1 v2 ⟩
+
 (** Steps *)
 | step_let xs v e1 e2 : ⟨ xs, ELet v e1 e2 ⟩ --> ⟨ (FLet v e2)::xs, e1 ⟩
 | step_app xs e el: ⟨ xs, EApp e el ⟩ --> ⟨ (FApp1 el)::xs, e ⟩
 | step_plus xs e1 e2 : ⟨ xs, EPlus e1 e2⟩ --> ⟨ (FPlus1 e2)::xs, e1⟩
 | step_if xs e1 e2 e3 : ⟨ xs, EIf e1 e2 e3⟩ --> ⟨ (FIf e2 e3)::xs, e1⟩
+
+(** Special step rules: need to "determinize them" *)
+| step_cons xs e1 e2 (H : ~VALCLOSED (ECons e1 e2)): ⟨ xs, ECons e1 e2 ⟩ --> ⟨ (FCons1 e1) :: xs, e2 ⟩
 where "⟨ fs , e ⟩ --> ⟨ fs' , e' ⟩" := (step fs e fs' e').
 
 Reserved Notation "⟨ fs , e ⟩ -[ k ]-> ⟨ fs' , e' ⟩" (at level 50).
@@ -203,7 +202,7 @@ Inductive step_rt : FrameStack -> Exp -> nat -> FrameStack -> Exp -> Prop :=
 where "⟨ fs , e ⟩ -[ k ]-> ⟨ fs' , e' ⟩" := (step_rt fs e k fs' e').
 
 Definition step_any (fs : FrameStack) (e : Exp) (v : Exp) : Prop :=
-  is_value v /\ exists k, ⟨fs, e⟩ -[k]-> ⟨[], v⟩.
+  VALCLOSED v /\ exists k, ⟨fs, e⟩ -[k]-> ⟨[], v⟩.
 
 Notation "⟨ fs , e ⟩ -->* v" := (step_any fs e v) (at level 50).
 
@@ -213,12 +212,12 @@ Proof.
 (*   Unshelve. cbn. constructor. *)
 Qed.
 
-Goal ⟨ [], simplefun 10 ⟩ -->* ELit 10.
+Local Goal ⟨ [], simplefun 10 ⟩ -->* ELit 10.
 Proof.
   repeat econstructor.
 Qed.
 
-Goal ⟨ [], simplefun2 10 10 ⟩ -->* ELit 20.
+Local Goal ⟨ [], simplefun2 10 10 ⟩ -->* ELit 20.
 Proof.
   unfold simplefun2.
   repeat econstructor.
@@ -226,14 +225,21 @@ Proof.
   all : try constructor.
 Qed.
 
-Goal ⟨ [], sum 1 ⟩ -->* ELit 1.
+Local Goal ⟨ [], sum 1 ⟩ -->* ELit 1.
 Proof.
+  assert (VALCLOSED (EFun [XVar]
+             (EIf (EVar 1) (EVar 1)
+                (EPlus (EVar 1) (EApp (EFunId 0) [EPlus (EVar 1) (ELit (-1))]))))). {
+    do 4 constructor.
+    1-4: repeat constructor. intros. inversion H; subst; cbn. 2: inversion H1.
+    repeat constructor.
+  }
   unfold sum.
   simpl.
   constructor. constructor. econstructor.
   econstructor.
   econstructor.
-  econstructor. constructor. cbn. econstructor. constructor. econstructor.
+  econstructor. constructor. cbn. econstructor. constructor. auto.
   econstructor.
   eapply red_app2. constructor.
   simpl. econstructor. econstructor. econstructor. eapply step_if.
@@ -241,8 +247,8 @@ Proof.
   econstructor. eapply step_plus.
   econstructor. eapply red_plus_left.
   econstructor. cbn. econstructor. eapply step_app.
-  econstructor. eapply red_app_start.
-  econstructor. econstructor.
+  econstructor. eapply red_app_start. auto.
+  econstructor.
   eapply step_plus.
 
   econstructor. eapply red_plus_left.
@@ -252,9 +258,18 @@ Proof.
   econstructor. eapply red_if_true.
   econstructor. eapply red_plus_right.
   econstructor.
+Qed.
 
-  Unshelve.
-  all : constructor.
+Local Goal ⟨[], ECons (EPlus (ELit 1) (ELit 1)) (ECons (ELit 1) (ECons (ELit 0) ENil))⟩ -->* ECons (ELit 2) (ECons (ELit 1) (ECons (ELit 0) ENil)).
+Proof.
+  split. repeat constructor. exists 6.
+  econstructor. constructor. intro. inversion H; inversion_is_value.
+  econstructor. constructor. repeat constructor.
+  econstructor. apply step_plus.
+  econstructor. constructor. constructor.
+  econstructor. constructor.
+  econstructor. constructor. 1-2: repeat constructor.
+  econstructor.
 Qed.
 
 Ltac proof_irr :=
@@ -267,31 +282,48 @@ Theorem step_determinism {e e' fs fs'} :
   ⟨ fs, e ⟩ --> ⟨fs', e'⟩ ->
   (forall fs'' e'', ⟨fs, e⟩ --> ⟨fs'', e''⟩ -> fs'' = fs' /\ e'' = e').
 Proof.
-  intro H. induction H; intros.
+  intro H. dependent induction H; intros.
   * inversion H0; subst; try inversion H; try (proof_irr; auto).
+    congruence.
   * inversion H; subst. auto.
   * inversion H0; subst; try inversion H'; try (proof_irr_many; auto).
+    congruence.
   * inversion H1; subst; try inversion H; auto.
+    congruence.
   * inversion H0; subst; auto; try inversion H.
+    congruence.
   * inversion H; subst; auto. congruence.
   * inversion H1; subst; auto; try congruence; try inversion H.
   * inversion H0; subst; try inversion H; try (proof_irr; auto).
+     congruence.
   * inversion H; subst. auto.
   * inversion H; subst; try inversion H0; try inversion H'; try inversion H1; try (proof_irr_many; auto).
+  * inversion H0; subst; try inversion_is_value. auto.
+    congruence.
+  * inversion H1; subst; try inversion_is_value. auto.
+    congruence.
   * inversion H; subst; try inversion H0; try inversion H'; try inversion H1; try (proof_irr_many; auto).
   * inversion H; subst; try inversion H0; try inversion H'; try inversion H1; try (proof_irr_many; auto).
   * inversion H; subst; try inversion H0; try inversion H'; try inversion H1; try (proof_irr_many; auto).
   * inversion H; subst; try inversion H0; try inversion H'; try inversion H1; try (proof_irr_many; auto).
+  * inversion H0; subst; try congruence. auto.
 Qed.
 
-Theorem value_nostep v (H : is_value v) :
+Theorem value_nostep v (H : VALCLOSED v) :
   forall fs' v', ⟨ [], v ⟩ --> ⟨fs' , v'⟩ -> False.
 Proof.
-  induction H; unfold not; intros; inversion H; inversion H0; inversion H1.
+  dependent induction H; intros.
+  * inversion H.
+  * inversion H1; subst. assert (VALCLOSED (ECons e1 v')) by (constructor; auto).
+    congruence.
+  * inversion H.
+  * inversion H.
+  * inversion H.
+  * inversion H0.
 Qed.
 
 Theorem step_rt_determinism {e v fs fs' k} :
-  ⟨fs, e⟩ -[k]-> ⟨fs', v⟩ -> is_value v
+  ⟨fs, e⟩ -[k]-> ⟨fs', v⟩ -> VALCLOSED v
 ->
   (forall fs'' v', ⟨fs, e⟩ -[k]-> ⟨fs'', v'⟩ -> fs' = fs'' /\ v' = v).
 Proof.
@@ -307,20 +339,19 @@ Theorem step_closedness : forall F e F' e',
 Proof.
   intros F e F' e' IH. induction IH; intros.
   * inversion H0. subst. inversion H4. inversion H3. subst. split; auto.
-    constructor; auto. constructor; auto. destruct v; inversion H; inversion H1; auto.
+    constructor; auto. constructor; auto.
   * inversion H. inversion H0. subst. split; auto. inversion H5. subst. cbn in H2.
     apply -> subst_preserves_scope_exp; eauto.
   * inversion H0. subst. inversion H5. inversion H9. subst. split; auto. constructor; auto.
     constructor; auto.
-    apply Forall_app. split; auto. constructor; auto. destruct v'; inversion H'; inversion H1; auto.
+    apply Forall_app. split; auto.
   * inversion H1. inversion H6. split. auto. subst. inversion H11.
     apply -> subst_preserves_scope_exp; eauto. subst.
     rewrite Nat.add_0_r. replace (S (length vl)) with (length (EFun vl e :: vs ++ [v])).
-    apply scoped_list_idsubst. constructor. auto. apply Forall_app. split; auto. constructor; auto.
-    destruct v; inversion H; inversion H3; auto. simpl. rewrite H0, app_length. simpl. lia.
+    apply scoped_list_idsubst. constructor. auto. apply Forall_app. split; auto.
+    simpl. rewrite H0, app_length. simpl. lia.
   * inversion H0. inversion H4. 
     subst. split; auto. apply -> subst_preserves_scope_exp; eauto.
-    apply cons_scope; auto. destruct val; inversion H; inversion H1; auto.
   * inversion H. inversion H3. subst. split; auto.
   * inversion H1. inversion H5. subst. split; auto.
   * inversion H0. inversion H4; subst. split; auto. constructor; auto.
@@ -328,16 +359,21 @@ Proof.
   * inversion H. inversion H3. subst. split; auto. constructor. constructor.
   * split; auto. inversion H0. 2: inversion H1. apply -> subst_preserves_scope_exp; eauto.
     subst. apply cons_scope; auto. constructor. auto.
+  * inversion H0. inversion H4. subst. split; auto. repeat constructor; auto.
+  * inversion H1. inversion H5. subst. split; auto. repeat constructor; auto.
   * inversion H0. 2: inversion H1. subst. split; auto. constructor; auto.
     now constructor.
   * inversion H0. 2: inversion H1. subst. split; auto. constructor; auto.
     constructor. rewrite indexed_to_forall. exact H4.
   * inversion H0. 2: inversion H1. subst. split; auto. constructor; auto. now constructor.
   * inversion H0. 2: inversion H1. subst. split; auto. constructor; auto. now constructor.
+  * inversion H1; subst; split; auto. 3: congruence.
+    all: constructor; auto; constructor; auto.
+    congruence.
 Qed.
 
-Theorem result_is_value_any (fs : FrameStack) (e v : Exp) :
-  ⟨ fs, e ⟩ -->* v -> is_value v.
+Theorem result_VALCLOSED_any (fs : FrameStack) (e v : Exp) :
+  ⟨ fs, e ⟩ -->* v -> VALCLOSED v.
 Proof.
   intros. destruct H. auto.
 Qed.
@@ -349,43 +385,47 @@ Corollary step_any_closedness : forall F e v,
 Proof.
   intros. destruct H, H2. induction H2.
   * destruct e; try inversion H; now inversion H1.
-  * apply step_closedness in H2; auto. now apply IHstep_rt.
+  * apply step_closedness in H2; auto.
 Qed.
 
 Definition terminates_sem (fs : FrameStack) (e : Exp) : Prop :=
   exists v, ⟨fs, e⟩ -->* v.
 
 Definition terminates_in_k_sem (fs : FrameStack) (e : Exp) (k : nat) : Prop :=
-  exists v, ⟨fs, e⟩ -[k]-> ⟨[], v⟩ /\ is_value v.
+  exists v, ⟨fs, e⟩ -[k]-> ⟨[], v⟩ /\ VALCLOSED v.
 
 
 
 Reserved Notation "| fs , e | k ↓" (at level 80).
 Inductive terminates_in_k : FrameStack -> Exp -> nat -> Prop :=
 
-| term_value v : is_value v -> | [] , v | 0 ↓
+| term_value v : VALCLOSED v -> | [] , v | 0 ↓
 | term_if_true fs e1 e2 k : | fs , e1 | k ↓ -> | (FIf e1 e2)::fs , ELit 0 | S k ↓
-| term_if_false fs e1 e2 v k : is_value v -> v <> ELit 0 -> | fs , e2 | k ↓ -> | (FIf e1 e2)::fs , v | S k ↓
-| term_plus_left e2 v fs (H : is_value v) k : | (FPlus2 v)::fs , e2 | k ↓ -> | (FPlus1 e2)::fs, v | S k ↓
+| term_if_false fs e1 e2 v k : VALCLOSED v -> v <> ELit 0 -> | fs , e2 | k ↓ -> | (FIf e1 e2)::fs , v | S k ↓
+| term_plus_left e2 v fs (H : VALCLOSED v) k : | (FPlus2 v)::fs , e2 | k ↓ -> | (FPlus1 e2)::fs, v | S k ↓
 | term_plus_right n m fs k : | fs , ELit (n + m) | k ↓ -> | (FPlus2 (ELit n))::fs, ELit m | S k ↓
-| term_let_subst v e2 fs k x : is_value v -> | fs, e2.[v/] | k ↓ -> | (FLet x e2)::fs, v | S k ↓
+| term_let_subst v e2 fs k x : VALCLOSED v -> | fs, e2.[v/] | k ↓ -> | (FLet x e2)::fs, v | S k ↓
 | term_letrec_subst vl b e fs f k : | fs, e.[EFun vl b/] | k ↓ -> | fs, ELetRec f vl b e | S k ↓
-| term_app_start v hd tl (H : is_value v) fs k : 
+| term_app_start v hd tl (H : VALCLOSED v) fs k : 
   | (FApp2 v tl [])::fs, hd| k ↓ -> | (FApp1 (hd::tl))::fs, v | S k ↓
 | term_app1 e fs k : | fs, e.[EFun [] e/] | k ↓ -> | (FApp1 [])::fs, EFun [] e | S k ↓
-| term_app_step v v' (H : is_value v) hd tl vs (H2 : Forall is_value vs) (H' : is_value v') fs k :
+| term_app_step v v' (H : VALCLOSED v) hd tl vs (H2 : Forall (fun v => VALCLOSED v) vs) (H' : VALCLOSED v') fs k :
   | (FApp2 v tl (vs ++ [v']))::fs, hd | k ↓ -> | (FApp2 v (hd::tl) vs)::fs , v' | S k ↓
 
-| term_app2 v vl e vs fs (H2 : Forall is_value vs) k :
-  length vl = S (length vs) -> is_value v -> | fs, e.[list_subst (EFun vl e  :: (vs ++ [v])) idsubst] | k ↓ 
+| term_app2 v vl e vs fs (H2 : Forall (fun v => VALCLOSED v) vs) k :
+  length vl = S (length vs) -> VALCLOSED v -> | fs, e.[list_subst (EFun vl e  :: (vs ++ [v])) idsubst] | k ↓ 
 -> | (FApp2 (EFun vl e) [] vs)::fs, v | S k ↓
-
+| term_cons1 e1 v2 fs k (H: VALCLOSED v2):
+  | FCons2 v2::fs, e1 | k ↓ -> | FCons1 e1 :: fs, v2 | S k ↓
+| term_cons2 v1 v2 fs k (H: VALCLOSED v2) (H0 : VALCLOSED v1):
+  | fs, ECons v1 v2 | k ↓ -> | FCons2 v2 :: fs, v1 | S k ↓
 
 | term_if e e1 e2 fs k : | (FIf e1 e2)::fs, e | k ↓ -> | fs, EIf e e1 e2 | S k ↓
 | term_plus e1 e2 fs k : | (FPlus1 e2)::fs, e1 | k ↓ -> | fs, EPlus e1 e2 | S k ↓
 | term_app e vs fs k : | (FApp1 vs)::fs, e | k ↓ -> | fs, EApp e vs | S k ↓
 | term_let v e1 e2 fs k : | (FLet v e2)::fs, e1 | k ↓ -> | fs, ELet v e1 e2 | S k ↓
-
+| term_cons fs e1 e2 k (H : ~VALCLOSED (ECons e1 e2)) :
+  | FCons1 e1 :: fs, e2 | k ↓ -> | fs, ECons e1 e2 | S k ↓
 where "| fs , e | k ↓" := (terminates_in_k fs e k).
 
 Definition terminates (fs : FrameStack) (e : Exp) := exists n, | fs, e | n ↓.
@@ -402,7 +442,8 @@ Proof.
     {
       inversion H. clear H. inversion H0; inversion H; subst.
       assert (terminates_in_k_sem fs' e' k). { econstructor. eauto. } apply IHk in H2.
-      clear H0. inversion H3; subst; econstructor; eauto.
+      clear H0. inversion H3; subst.
+      all: try econstructor; eauto.
     }
     {
       inversion H; subst;
@@ -456,7 +497,7 @@ Proof.
   * destruct H. inversion H. subst. apply value_nostep in H0; intuition.
   * destruct H.
     inversion H. subst. apply (step_determinism H0) in H3. destruct H3. subst.
-    assert (exists y, ⟨ fs', e' ⟩ -[ n ]-> ⟨ [], y ⟩ /\ is_value y). { 
+    assert (exists y, ⟨ fs', e' ⟩ -[ n ]-> ⟨ [], y ⟩ /\ VALCLOSED y). { 
       eexists. eauto. }
     apply ex_intro in H6. apply terminates_in_k_eq_terminates_in_k_sem in H2.
     now rewrite Nat.sub_1_r.
@@ -480,126 +521,6 @@ Proof.
   * rewrite Nat.sub_0_r. auto.
   * apply terminates_step_2 with (n := n) in H2; auto.
     eapply IHk in H5; auto. 2: exact H2. now replace (n - S k) with ((n - 1) - k) by lia.
-Qed.
-
-Theorem is_value_dec v :
-  {is_value v} + {~is_value v}.
-Proof.
-  destruct v.
-  1, 4: left; constructor.
-  all: right; intro; inversion H.
-Qed.
-
-Theorem term_dec :
-  forall k e Fs, | Fs, e | k ↓ \/ ~ | Fs, e | k ↓.
-Proof.
-  induction k using lt_wf_ind. intros.
-  destruct k.
-  * destruct Fs.
-    - destruct e. 1, 4: left; do 2 constructor.
-      all: right; intro; inversion H0; inversion H1.
-    - right. intro. inversion H0.
-  * destruct e.
-    - destruct Fs. right. intro. inversion H0.
-      destruct f.
-      + destruct l0.
-        ** right. intro. inversion H0.
-        ** epose proof (H k ltac:(lia) e _). destruct H0.
-           -- left. constructor. constructor. exact H0.
-           -- right. intro. inversion H1. subst. contradiction.
-      + destruct l1.
-        ** destruct v.
-           1-3, 5-9: right; intro; inversion H0.
-           destruct (Nat.eq_dec (length vl) (S (length l2))).
-           -- destruct (Forall_dec is_value is_value_dec l2).
-              ++ epose proof (H k ltac:(lia) _ _). destruct H0.
-                 *** left. constructor; auto. constructor. exact H0.
-                 *** right. intro. inversion H1. contradiction.
-              ++ right. intro. inversion H0. contradiction.
-           -- right. intro. inversion H0. subst. contradiction.
-        ** destruct (Forall_dec is_value is_value_dec l2).
-           -- destruct (is_value_dec v).
-              ++ epose proof (H k ltac:(lia) _ _). destruct H0.
-                 *** left. constructor; auto. constructor. exact H0.
-                 *** right. intro. inversion H1. contradiction.
-              ++ right. intro. inversion H0. contradiction.
-           -- right. intro. inversion H0. contradiction.
-      + epose proof (H k ltac:(lia) _ _). destruct H0.
-        ** left. constructor. constructor. exact H0.
-        ** right. intro. inversion H1. contradiction.
-      + epose proof (H k ltac:(lia) _ _). destruct H0.
-        ** left. constructor. constructor. exact H0.
-        ** right. intro. inversion H1. contradiction.
-      + destruct v.
-        2-9: right; intro; inversion H0.
-        ** epose proof (H k ltac:(lia) _ _). destruct H0.
-           -- left. constructor. exact H0.
-           -- right. intro. inversion H1. contradiction.
-      + destruct l.
-        ** epose proof (H k ltac:(lia) _ _). destruct H0.
-           -- left. constructor. exact H0.
-           -- right. intro. inversion H1. contradiction. contradiction.
-        ** epose proof (H k ltac:(lia) _ _). destruct H0.
-           -- left. constructor. constructor. intro. inversion H1. exact H0.
-           -- right. intro. inversion H1. contradiction.
-        ** epose proof (H k ltac:(lia) _ _). destruct H0.
-           -- left. constructor. constructor. intro. inversion H1. exact H0.
-           -- right. intro. inversion H1. contradiction.
-    - right. intro. inversion H0; inversion_is_value.
-    - right. intro. inversion H0; inversion_is_value.
-    - destruct Fs. right. intro. inversion H0.
-      destruct f.
-      + destruct l.
-        ** destruct vl.
-           -- epose proof (H k ltac:(lia) _ _). destruct H0.
-              ++ left. constructor. exact H0.
-              ++ right. intro. inversion H1. contradiction.
-           -- right. intro. inversion H0.
-        ** epose proof (H k ltac:(lia) _ _). destruct H0.
-           -- left. constructor. constructor. exact H0.
-           -- right. intro. inversion H1. subst. contradiction.
-      + destruct l1.
-        ** destruct v.
-           1-3, 5-9: right; intro; inversion H0.
-           destruct (Nat.eq_dec (length vl0) (S (length l2))).
-           -- destruct (Forall_dec is_value is_value_dec l2).
-              ++ epose proof (H k ltac:(lia) _ _). destruct H0.
-                 *** left. constructor; auto. constructor. exact H0.
-                 *** right. intro. inversion H1. contradiction.
-              ++ right. intro. inversion H0. contradiction.
-           -- right. intro. inversion H0. subst. contradiction.
-        ** destruct (Forall_dec is_value is_value_dec l2).
-           -- destruct (is_value_dec v).
-              ++ epose proof (H k ltac:(lia) _ _). destruct H0.
-                 *** left. constructor; auto. constructor. exact H0.
-                 *** right. intro. inversion H1. contradiction.
-              ++ right. intro. inversion H0. contradiction.
-           -- right. intro. inversion H0. contradiction.
-      + epose proof (H k ltac:(lia) _ _). destruct H0.
-        ** left. constructor. constructor. exact H0.
-        ** right. intro. inversion H1. contradiction.
-      + epose proof (H k ltac:(lia) _ _). destruct H0.
-        ** left. constructor. constructor. exact H0.
-        ** right. intro. inversion H1. contradiction.
-      + right. intro. inversion H0.
-      + epose proof (H k ltac:(lia) _ _). destruct H0.
-        ** left. constructor. constructor. congruence. exact H0.
-        ** right. intro. inversion H1. contradiction.
-    - epose proof (H k ltac:(lia) _ _). destruct H0.
-      + left. constructor. exact H0.
-      + right. intro. inversion H1; try inversion_is_value. contradiction.
-    - epose proof (H k ltac:(lia) _ _). destruct H0.
-      + left. constructor. exact H0.
-      + right. intro. inversion H1; try inversion_is_value. contradiction.
-    - epose proof (H k ltac:(lia) _ _). destruct H0.
-      + left. constructor. exact H0.
-      + right. intro. inversion H1; try inversion_is_value. contradiction.
-    - epose proof (H k ltac:(lia) _ _). destruct H0.
-      + left. constructor. exact H0.
-      + right. intro. inversion H1; try inversion_is_value. contradiction.
-    - epose proof (H k ltac:(lia) _ _). destruct H0.
-      + left. constructor. exact H0.
-      + right. intro. inversion H1; try inversion_is_value. contradiction.
 Qed.
 
 Corollary transitive_eval : forall n  Fs Fs' e e',
@@ -635,58 +556,59 @@ Proof.
 Qed.
 
 Lemma eval_app_partial :
-  forall vals vl e v Fs hds, length vl = length (hds ++ v :: vals) ->
-  Forall is_value vals -> Forall is_value hds -> is_value v ->
+  forall vals vl e v Fs hds (P : VALCLOSED (EFun vl e)), length vl = length (hds ++ v :: vals) ->
+  Forall (fun v => VALCLOSED v) vals -> Forall (fun v => VALCLOSED v) hds -> VALCLOSED v ->
   ⟨ FApp2 (EFun vl e) vals hds :: Fs, v ⟩ -[S (length vals)]-> ⟨ Fs , e.[list_subst (EFun vl e :: (hds ++ v :: vals)) idsubst]⟩.
 Proof.
   induction vals; intros.
   * simpl. econstructor. constructor; auto. rewrite app_length in H. simpl in H. lia.
     constructor.
-  * simpl. econstructor. constructor; auto. constructor. inversion H0. subst.
-    epose proof (IHvals vl e a _ (hds ++ [v]) _ H6 _ H5). rewrite <- app_assoc in H3.
+  * simpl. econstructor. constructor; auto. inversion H0. subst.
+    epose proof (IHvals vl e a _ (hds ++ [v]) _ _ H6 _ H5). rewrite <- app_assoc in H3.
     exact H3.
   Unshelve.
+    auto.
     rewrite <- app_assoc. auto. apply Forall_app. split. auto. constructor; auto.
 Qed.
 
 Lemma app1_eval :
-  forall vals Fs vl e, Forall is_value vals -> length vl = length vals ->
+  forall vals Fs vl e (P : VALCLOSED (EFun vl e)), Forall (fun v => VALCLOSED v) vals -> length vl = length vals ->
   exists k : nat,
   ⟨ [FApp1 vals] ++ Fs, EFun vl e ⟩ -[ k ]-> ⟨ Fs, e.[EFun vl e .: list_subst vals idsubst] ⟩.
 Proof.
   destruct vals; intros.
   * apply length_zero_iff_nil in H0. subst. exists 1. econstructor.
     simpl. constructor. cbn. constructor.
-  * exists (S (S (length vals))). simpl. econstructor. do 2 constructor.
+  * exists (S (S (length vals))). simpl. econstructor. constructor. auto.
     inversion H. subst.
     apply eval_app_partial; auto.
 Qed.
 
 Lemma eval_app_partial_core :
-  forall hds' vals vl e e' v Fs hds, (* length vl = length (hds ++ v::hds' ++ vals) -> *)
-  Forall is_value hds -> Forall is_value hds' -> is_value v ->
+  forall hds' vals vl e e' v Fs hds (P : VALCLOSED (EFun vl e)), (* length vl = length (hds ++ v::hds' ++ vals) -> *)
+  Forall (fun v => VALCLOSED v) hds -> Forall (fun v => VALCLOSED v) hds' -> VALCLOSED v ->
   ⟨ FApp2 (EFun vl e) (hds' ++ e' :: vals) hds :: Fs, v ⟩ -[S (length hds')]-> 
   ⟨ FApp2 (EFun vl e) vals (hds ++ v :: hds') :: Fs , e'⟩.
 Proof.
   induction hds'; intros.
   * simpl. econstructor. constructor; auto. constructor.
-    constructor.
-  * simpl. econstructor. constructor; auto. constructor. inversion H0. subst.
-    epose proof (IHhds' vals vl e _ a Fs (hds ++ [v]) _ _ H4).
+  * simpl. econstructor. constructor; auto. inversion H0. subst.
+    epose proof (IHhds' vals vl e _ a Fs (hds ++ [v]) _ _ _ H4).
     rewrite <- app_assoc in H2. exact H2.
   Unshelve.
+    auto.
     apply Forall_app. split; auto. auto.
 Qed.
 
-Lemma full_eval_app_partial : forall e vals vl Fs,
-  length vl = length vals -> Forall is_value vals ->
+Lemma full_eval_app_partial : forall e vals vl Fs (P : VALCLOSED (EFun vl e)),
+  length vl = length vals -> Forall (fun v => VALCLOSED v) vals ->
   ⟨ Fs, EApp (EFun vl e) vals ⟩ -[2 + length vals]-> ⟨ Fs, e.[EFun vl e .: list_subst vals idsubst] ⟩.
 Proof.
   destruct vals; intros.
   - simpl. apply length_zero_iff_nil in H. subst. econstructor. constructor.
     econstructor. constructor. constructor.
   - simpl. econstructor. constructor.
-    econstructor. constructor. constructor. inversion H0.
+    econstructor. constructor. auto. inversion H0.
     apply eval_app_partial; auto.
 Qed.
 
@@ -704,13 +626,14 @@ Proof.
     apply IHIH in H5. auto.
 Qed.
 
-Theorem app_term_fun : forall tl k hds e e' Fs,
-  | FApp2 e' tl hds :: Fs, e | k ↓ -> Forall is_value hds ->
+Theorem app_term_fun : forall tl k hds e e' Fs (P : EXPCLOSED e)   (PP : Forall (fun v => EXPCLOSED v) tl),
+  | FApp2 e' tl hds :: Fs, e | k ↓ ->
+  Forall (fun v => VALCLOSED v) hds ->
   (forall m : nat,
     m < S k ->
     forall (Fs : FrameStack) (e : Exp),
-    | Fs, e | m ↓ ->
-    exists (v : Exp) (k : nat), is_value v /\ ⟨ Fs, e ⟩ -[ k ]-> ⟨ Fs, v ⟩)
+    EXPCLOSED e -> | Fs, e | m ↓ ->
+    exists (v : Exp) (k : nat), VALCLOSED v /\ ⟨ Fs, e ⟩ -[ k ]-> ⟨ Fs, v ⟩)
 ->
   exists vl b, e' = EFun vl b /\ length vl = S (length (hds ++ tl)).
 Proof.
@@ -719,15 +642,18 @@ Proof.
     eapply terminates_step_any_2 in H. 2: exact H3.
     inversion H; subst; try inversion_is_value.
     rewrite app_length, Nat.add_0_r. do 2 eexists. split. reflexivity. auto.
-  * apply H1 in H as H'. 2: lia. destruct H', H2, H2.
+    congruence. auto.
+  * apply H1 in H as H'; auto. destruct H', H2, H2.
     eapply terminates_step_any_2 in H. 2: exact H3.
-    inversion H; subst; try inversion_is_value.
+    inversion H; subst; try inversion_is_value. 2: congruence.
     apply H1 in H13 as H''. 2: lia. destruct H'', H4, H4.
     eapply terminates_step_any_2 in H13. 2: exact H5.
     apply IHtl in H13. destruct H13, H6, H6. subst. exists x3, x4. split; auto.
     repeat rewrite app_length in *. simpl in *. lia.
-    apply Forall_app; auto.
-    intros. eapply H1. 2: exact H7. lia.
+    3: apply Forall_app; auto.
+    2,4: inversion PP; auto.
+    constructor. auto.
+    intros. eapply H1. 3: exact H8. lia. auto.
 Qed.
 
 Theorem frame_indep_step : forall e F F' Fs e',
@@ -777,33 +703,35 @@ Lemma term_app_length : forall tl hds e k Fs x0,
     m < S k ->
     forall (Fs : FrameStack) (e : Exp),
     | Fs, e | m ↓ ->
-    exists (v : Exp) (k : nat), is_value v /\ ⟨ Fs, e ⟩ -[ k ]-> ⟨ Fs, v ⟩ /\ k <= m) ->
+    exists (v : Exp) (k : nat), VALCLOSED v /\ ⟨ Fs, e ⟩ -[ k ]-> ⟨ Fs, v ⟩ /\ k <= m) ->
   | FApp2 x0 tl hds :: Fs, e | k ↓ -> k > length tl.
 Proof.
   induction tl; intros.
   * inversion H0; simpl; lia.
   * simpl. apply H in H0 as H0'. destruct H0', H1, H1, H2.
     eapply (terminates_step_any_2 _ _ _ _ H0) in H2 as H2'.
-    inversion H2'; subst; try inversion_is_value. 2: lia.
-    eapply IHtl in H13. lia. intros. apply H. lia. auto.
+    inversion H2'; subst; try inversion_is_value. 3: lia.
+    eapply IHtl in H13. lia. intros. apply H. lia. auto. congruence.
 Qed.
 
 Lemma eval_app_partial_core_2 :
-  forall hds' vals vl e e' v Fs hds k,
+  forall hds' vals vl e e' v Fs hds k (P : VALCLOSED (EFun vl e)) (PP : Forall (fun v => EXPCLOSED v) hds'),
   (forall m : nat,
     m < S k ->
     forall (Fs : FrameStack) (e : Exp),
-    | Fs, e | m ↓ -> exists (v : Exp) (k : nat), is_value v /\ ⟨ Fs, e ⟩ -[ k ]-> ⟨ Fs, v ⟩) ->
+    EXPCLOSED e -> | Fs, e | m ↓ ->
+    exists (v : Exp) (k : nat), VALCLOSED v /\ ⟨ Fs, e ⟩ -[ k ]-> ⟨ Fs, v ⟩) ->
   | FApp2 (EFun vl e) (hds' ++ e' :: vals) hds :: Fs, v | k ↓ ->
-  is_value v ->
-  Forall is_value hds ->
-  exists k0 hds'', k0 <= k /\ Forall is_value hds'' /\
+  VALCLOSED v ->
+  Forall (fun v => VALCLOSED v) hds ->
+  exists k0 hds'', k0 <= k /\ Forall (fun v => VALCLOSED v) hds'' /\
   ⟨ FApp2 (EFun vl e) (hds' ++ e' :: vals) hds :: Fs, v ⟩ -[k0]-> 
   ⟨ FApp2 (EFun vl e) vals (hds ++ v :: hds'') :: Fs , e'⟩.
 Proof.
   induction hds'; intros.
   * simpl in *. inversion H0; subst; try inversion_is_value.
     exists 1, []. split. lia. split. auto. econstructor. constructor; auto. constructor.
+    congruence.
   * simpl in *. inversion H0; subst; try inversion_is_value.
     apply H in H12 as P1. 2: lia. destruct P1, H3, H3.
     eapply (terminates_step_any_2 _ _ _ _ H12) in H4 as H4'.
@@ -813,13 +741,13 @@ Proof.
     - simpl in H4.
       assert (⟨ FApp2 (EFun vl e) (e' :: vals) (hds ++ [v]) :: Fs, x ⟩ -[1]->
            ⟨ FApp2 (EFun vl e) vals ((hds ++ [v]) ++ [x]) :: Fs, e' ⟩).
-           { repeat econstructor; auto. }
+           { do 2 econstructor; auto. }
       epose proof (transitive_eval _ _ _ _ _ H4 _ _ _ H5).
       exists (S (x0 + 1)), [x]. split. lia. split. auto.
       econstructor. constructor; auto.
       rewrite <- app_assoc in H7. simpl in H7. auto.
-    - epose proof (IHhds' vals vl e e' x Fs _ _ _ H4' H'0 H15).
-      Unshelve. 2: { intros. eapply H. 2: exact H7. lia. }
+    - epose proof (IHhds' vals vl e e' x Fs _ _ _ _ _ H4' H'0 H15).
+      Unshelve. 4: { intros. eapply H. 3: exact H8. lia. auto. }
       destruct H5, H5, H5, H7.
       epose proof (transitive_eval _ _ _ _ _ H4 _ _ _ H8).
       exists (S (x0 + x1)), (x::x2). 
@@ -830,10 +758,15 @@ Proof.
         replace ((hds ++ [v]) ++ x :: x2) with (hds ++ v :: x :: x2) in H9.
         exact H9.
         rewrite <- app_assoc. auto.
+      + auto.
+      + now inversion PP.
+    - congruence.
+    - now inversion PP.
+    - congruence.
 Qed.
 
-Theorem term_eval : forall x Fs e, | Fs, e | x ↓ ->
-  exists v k, is_value v /\ ⟨ Fs, e ⟩ -[k]-> ⟨ Fs, v ⟩ (* /\ k <= x *).
+Theorem term_eval : forall x Fs e (P : EXPCLOSED e), | Fs, e | x ↓ ->
+  exists v k, VALCLOSED v /\ ⟨ Fs, e ⟩ -[k]-> ⟨ Fs, v ⟩ (* /\ k <= x *).
 Proof.
   induction x using lt_wf_ind. destruct x; intros; inversion H0; subst; try congruence.
   * exists e, 0. now repeat constructor.
@@ -844,9 +777,14 @@ Proof.
   * exists e, 0. split; [ auto | now constructor].
   * apply H in H4. destruct H4, H1, H1. exists x0, (S x1).
     split; [ auto | ]. econstructor. constructor. auto. lia.
+    inversion P. 2: inversion_is_value. subst.
+     apply -> subst_preserves_scope_exp; eauto.
+    apply cons_scope; auto. now constructor.
   * exists e, 0. split; [ auto | now constructor ].
-  * exists (EFun [] e0), 0. split; [ constructor | do 2 constructor].
+  * exists (EFun [] e0), 0. inversion P. split; [ auto | do 2 constructor].
   * exists e, 0. split; [ auto | now constructor].
+  * exists e, 0. split; [ auto | now constructor ].
+  * exists e, 0. split; [ auto | now constructor ].
   * exists e, 0. split; [ auto | now constructor ].
   * apply H in H4 as HH. destruct HH, H1, H1. 2: lia.
     eapply (terminates_step_any_2 _ _ _ _ H4) in H2 as H2'.
@@ -854,11 +792,13 @@ Proof.
     - apply H in H8. 2: lia. destruct H8, H3, H3.
       exists x0, (S (x1 + S x2)). split. auto.
       econstructor. constructor. eapply transitive_eval; eauto.
-      econstructor. constructor. auto.
+      econstructor. constructor. auto. now inversion P.
     - apply H in H11. 2: lia. destruct H11, H3, H3.
       exists x2, (S (x1 + S x3)). split. auto.
       econstructor. constructor. eapply transitive_eval; eauto.
-      econstructor. constructor; auto. auto.
+      econstructor. constructor; auto. auto. now inversion P.
+    - congruence.
+    - now inversion P.
   * apply H in H4 as HH. destruct HH, H1, H1. 2: lia.
     eapply (terminates_step_any_2 _ _ _ _ H4) in H2 as H2'.
     inversion H2'; subst; try inversion_is_value.
@@ -870,6 +810,11 @@ Proof.
     econstructor. constructor. eapply transitive_eval; eauto. 
     econstructor. constructor; auto. eapply transitive_eval; eauto.
     econstructor. constructor. constructor.
+
+    congruence.
+    now inversion P.
+    congruence.
+    now inversion P.
   * apply H in H4 as v_eval. 2: lia. destruct v_eval, H1, H1.
     eapply (terminates_step_any_2 _ _ _ _ H4) in H2 as H2'.
     destruct vs.
@@ -878,56 +823,74 @@ Proof.
       exists x0, (S (x1 + S x2)). split; auto.
       econstructor. constructor. eapply transitive_eval; eauto.
       econstructor. constructor. auto.
+      inversion H1. subst. apply -> subst_preserves_scope_exp; eauto.
+      congruence.
     - inversion H2'; subst; try inversion_is_value.
-      
       assert (| FApp2 x0 vs [] :: Fs, e | k ↓) as PP by auto.
       eapply H in H10. 2: lia. destruct H10, H3, H3.
-      destruct (length vs) eqn:P.
-      + apply length_zero_iff_nil in P. subst.
+      destruct (length vs) eqn:P0.
+      + apply length_zero_iff_nil in P0. subst.
         eapply (terminates_step_any_2 _ _ _ _ PP) in H5 as H5'.
         inversion H5'; subst; try inversion_is_value.
         apply H in H16. 2: lia. destruct H16, H6, H6.
         assert (⟨ FApp2 (EFun vl e1) [] [] :: Fs, x2 ⟩ -[1]-> ⟨ Fs, e1.[list_subst (EFun vl e1 :: [] ++ [x2]) idsubst] ⟩).
         { repeat econstructor; auto. }
         epose proof (transitive_eval _ _ _ _ _ H10 _ _ _ H7).
-        assert (⟨ FApp1 [e] :: Fs, EFun vl e1 ⟩ -[1]-> ⟨ FApp2 (EFun vl e1) [] [] :: Fs, e ⟩). { repeat econstructor. }
+        assert (⟨ FApp1 [e] :: Fs, EFun vl e1 ⟩ -[1]-> ⟨ FApp2 (EFun vl e1) [] [] :: Fs, e ⟩). { do 2 econstructor. auto. }
         epose proof (transitive_eval _ _ _ _ _ H2 _ _ _ H16).
         epose proof (transitive_eval _ _ _ _ _ H5 _ _ _ H10).
         epose proof (transitive_eval _ _ _ _ _ H17 _ _ _ H18).
         epose proof (transitive_eval _ _ _ _ _ H19 _ _ _ H7).
         exists x0, (S (x1 + 1 + (x3 + 1) + x4)). split; auto.
         econstructor. constructor. auto.
-      + apply eq_sym, last_element_exists in P. destruct P, H6. subst.
+        inversion H1. subst. apply -> subst_preserves_scope_exp; eauto.
+        2: congruence.
+        cbn. apply cons_scope; auto. rewrite H14. apply cons_scope; auto.
+      + apply eq_sym, last_element_exists in P0. destruct P0, H6. subst.
         eapply (terminates_step_any_2 _ _ _ _ PP) in H5 as H5'.
-        inversion H8.
         
-        apply app_term_fun in H5'; auto.
-        destruct H5', H7, H7. subst. congruence. shelve.
+        apply app_term_fun in H5' as H5''; auto.
+        destruct H5'', H6, H6. subst.
         
         subst.
-        epose proof (eval_app_partial_core_2 x4 [] vl e1 x5 _ _ _ _ _ H5' H3 ltac:(auto)). destruct H6, H6, H6, H7. simpl in H10.
-        eapply (terminates_step_any_2 _ _ _ _ H5') in H10 as H7'.
-        apply H in H7' as H7''. 2: lia. destruct H7'', H11, H11.
-        eapply (terminates_step_any_2 _ _ _ _ H7') in H12 as H11'.
+        epose proof (eval_app_partial_core_2 x4 [] x6 x7 x5 x2 Fs _ _ H8 _ _ H5' H3 ltac:(auto)). destruct H6, H6, H6, H10. simpl in H11.
+        eapply (terminates_step_any_2 _ _ _ _ H5') in H11 as H7'.
+        apply H in H7' as H7''. 2: lia. destruct H7'', H12, H12.
+        eapply (terminates_step_any_2 _ _ _ _ H7') in H13 as H11'.
         inversion H11'; subst; try inversion_is_value.
-        apply H in H22. 2: lia. destruct H22, H13, H13.
-        epose proof (transitive_eval _ _ _ _ _ H10 _ _ _ H12).
-        assert (⟨ FApp2 (EFun vl e1) [] (x2 :: x6) :: Fs, x7 ⟩ -[1]->
-              ⟨ Fs, e1.[list_subst (EFun vl e1 :: (x2 :: x6) ++ [x7]) idsubst] ⟩). { econstructor. constructor; auto. constructor. }
-        epose proof (transitive_eval _ _ _ _ _ H15 _ _ _ H16).
-        epose proof (transitive_eval _ _ _ _ _ H18 _ _ _ H14).
-        clear H15 H16 H14 H18.
-        epose proof (transitive_eval _ _ _ _ _ H5 _ _ _ H22).
-        assert (⟨ FApp1 (e :: x4 ++ [x5]) :: Fs, EFun vl e1 ⟩ -[1]->
-            ⟨ FApp2 (EFun vl e1) (x4 ++ [x5]) [] :: Fs, e ⟩).
-            { econstructor. constructor. constructor. constructor. }
-        epose proof (transitive_eval _ _ _ _ _ H15 _ _ _ H14).
-        epose proof (transitive_eval _ _ _ _ _ H2 _ _ _ H16).
+        apply H in H23. 2: lia. destruct H23, H14, H14.
+        epose proof (transitive_eval _ _ _ _ _ H11 _ _ _ H13).
+        assert (⟨ FApp2 (EFun x6 x7) [] (x2 :: x8) :: Fs, x9 ⟩ -[1]->
+              ⟨ Fs, x7.[list_subst (EFun x6 x7 :: (x2 :: x8) ++ [x9]) idsubst] ⟩). { econstructor. constructor; auto. constructor. }
+        epose proof (transitive_eval _ _ _ _ _ H16 _ _ _ H17).
+        epose proof (transitive_eval _ _ _ _ _ H19 _ _ _ H15).
+        clear H17 H16 H15 H19.
+        epose proof (transitive_eval _ _ _ _ _ H5 _ _ _ H23).
+        assert (⟨ FApp1 (e :: x4 ++ [x5]) :: Fs, EFun x6 x7 ⟩ -[1]->
+            ⟨ FApp2 (EFun x6 x7) (x4 ++ [x5]) [] :: Fs, e ⟩).
+            { econstructor. constructor. auto. constructor. }
+        epose proof (transitive_eval _ _ _ _ _ H16 _ _ _ H15).
+        epose proof (transitive_eval _ _ _ _ _ H2 _ _ _ H17).
         
-        exists x9, (S (x1 + (1 + (x3 + (x0 + x8 + 1 + x10))))). split; auto.
+        exists x11, (S (x1 + (1 + (x3 + (x0 + x10 + 1 + x12))))). split; auto.
         econstructor. constructor. auto.
-     Unshelve.
-       all : intros; eapply H. 2: exact H10. 3: exact H7. all: lia.
+
+        2: congruence.
+        2: { inversion P. 2: inversion_is_value. 
+             subst. rewrite <- indexed_to_forall in H15.
+             inversion H15. subst. rewrite Forall_app in H17. destruct H17.
+             now inversion H13. }
+        ** inversion H1. apply -> subst_preserves_scope_exp; eauto.
+           replace (S (Datatypes.length x6) + 0) with (length ((EFun x6 x7 :: (x2 :: x8) ++ [x9]))). 2: { simpl. rewrite app_length. simpl in *. lia. }
+           apply scoped_list_idsubst. simpl. do 2 constructor; auto.
+           apply Forall_app; auto.
+        ** constructor. auto.
+        ** inversion P. subst. rewrite <- indexed_to_forall in H11.
+            now inversion H11. inversion_is_value.
+        ** intros. eapply H. 3: exact H10. lia. auto.
+      + inversion P. subst. apply (H7 0). simpl. lia. inversion_is_value.
+      + congruence.
+    - now inversion P.
   * apply H in H4 as HH. destruct HH, H1, H1. 2: lia.
     eapply (terminates_step_any_2 _ _ _ _ H4) in H2 as H2'.
     inversion H2'; subst; try inversion_is_value.
@@ -937,34 +900,57 @@ Proof.
     split. auto.
     econstructor. constructor. eapply transitive_eval; eauto. 
     econstructor. constructor; auto. auto.
+    2: congruence.
+    inversion P. 2: inversion_is_value. apply -> subst_preserves_scope_exp; eauto.
+    now inversion P.
+  * apply H in H5 as HH. 2: lia. 2: now inversion P.
+    destruct HH as [v2 [k2 [V2CL Eval2]]].
+    eapply (terminates_step_any_2 _ _ _ _ H5) in Eval2 as Eval2'.
+    inversion Eval2'; subst; try inversion_is_value. 2: congruence.
+    apply H in H8 as [v1 [k1 [V1CL Eval1]]]. 2: lia. 2: now inversion P.
+    assert (⟨ FCons1 e1 :: Fs, v2 ⟩ -[1]-> ⟨ FCons2 v2 :: Fs, e1 ⟩).
+    { econstructor. constructor. auto. constructor. }
+    eapply transitive_eval in H1. 2: exact Eval2.
+    eapply transitive_eval in Eval1. 2: exact H1.
+    assert (⟨ FCons2 v2 :: Fs, v1 ⟩ -[1]-> ⟨ Fs, ECons v1 v2 ⟩).
+    { econstructor. constructor; auto. constructor. }
+    eapply transitive_eval in H3. 2: exact Eval1.
+    exists (ECons v1 v2), (S ((k2 + 1 + k1) + 1)). split. constructor; auto.
+    econstructor. constructor; auto. exact H3.
+    Unshelve.
+    - inversion P. subst. rewrite <- indexed_to_forall in H12. inversion H12.
+      subst. now rewrite Forall_app in H14. inversion_is_value.
+    - intros. eapply H. 3: exact H11. lia. auto.
 Qed.
 
 Corollary app_term_fun_final : forall tl k hds e e' Fs,
-  | FApp2 e' tl hds :: Fs, e | k ↓ -> Forall is_value hds
+  | FApp2 e' tl hds :: Fs, e | k ↓ -> Forall (fun v => VALCLOSED v) hds ->
+  EXPCLOSED e -> Forall (fun e => EXPCLOSED e) tl
 ->
   exists vl b, e' = EFun vl b /\ length vl = S (length (hds ++ tl)).
 Proof.
   intros. eapply app_term_fun; eauto.
-  intros. eapply term_eval. eauto.
+  intros. eapply term_eval. eauto. eauto.
 Qed.
 
 Lemma eval_app_partial_core_emtpy :
-  forall hds' vals vl e e' v Fs hds k,
+  forall hds' vals vl e e' v Fs hds k (P : EXPCLOSED (EFun vl e)) (PP : Forall (fun v => EXPCLOSED v) hds'),
   (forall m : nat,
     m < S k ->
     forall (Fs : FrameStack) (e : Exp),
-    | Fs, e | m ↓ -> exists (v : Exp) (k : nat), is_value v /\ ⟨ [], e ⟩ -[ k ]-> ⟨ [], v ⟩) ->
+    EXPCLOSED e -> | Fs, e | m ↓ 
+    -> exists (v : Exp) (k : nat), VALCLOSED v /\ ⟨ [], e ⟩ -[ k ]-> ⟨ [], v ⟩) ->
   | FApp2 (EFun vl e) (hds' ++ e' :: vals) hds :: Fs, v | k ↓ ->
-  is_value v ->
-  Forall is_value hds ->
-  exists k0 hds'', k0 <= k /\ Forall is_value hds'' /\
+  VALCLOSED v ->
+  Forall (fun v => VALCLOSED v) hds ->
+  exists k0 hds'', k0 <= k /\ Forall (fun v => VALCLOSED v) hds'' /\
   ⟨ [FApp2 (EFun vl e) (hds' ++ e' :: vals) hds], v ⟩ -[k0]-> 
   ⟨ [FApp2 (EFun vl e) vals (hds ++ v :: hds'')] , e'⟩.
 Proof.
   induction hds'; intros.
-  * simpl in *. inversion H0; subst; try inversion_is_value.
+  * simpl in *. inversion H0; subst; try inversion_is_value. 2: congruence.
     exists 1, []. split. lia. split. auto. econstructor. constructor; auto. constructor.
-  * simpl in *. inversion H0; subst; try inversion_is_value.
+  * simpl in *. inversion H0; subst; try inversion_is_value. 2: congruence.
     apply H in H12 as P1. 2: lia. destruct P1, H3, H3.
     eapply frame_indep_nil in H4 as H4_1.
     eapply (terminates_step_any_2 _ _ _ _ H12) in H4_1 as H4'.
@@ -974,14 +960,14 @@ Proof.
     - simpl in H4.
       assert (⟨ [FApp2 (EFun vl e) (e' :: vals) (hds ++ [v])], x ⟩ -[1]->
            ⟨ [FApp2 (EFun vl e) vals ((hds ++ [v]) ++ [x])], e' ⟩).
-           { repeat econstructor; auto. }
+           { do 2 econstructor; auto. }
       eapply frame_indep_nil in H4.
       epose proof (transitive_eval _ _ _ _ _ H4 _ _ _ H5).
       exists (S (x0 + 1)), [x]. split. lia. split. auto.
       econstructor. constructor; auto.
       rewrite <- app_assoc in H7. simpl in H7. auto.
-    - epose proof (IHhds' vals vl e e' x Fs _ _ _ H4' H'0 H15).
-      Unshelve. 2: { intros. eapply H. 2: exact H7. lia. }
+    - epose proof (IHhds' vals vl e e' x Fs _ _ _ _ _ H4' H'0 H15).
+      Unshelve. 4: { intros. eapply H. 3: exact H8. lia. auto. }
       destruct H5, H5, H5, H7.
       eapply frame_indep_nil in H4.
       epose proof (transitive_eval _ _ _ _ _ H4 _ _ _ H8).
@@ -993,10 +979,14 @@ Proof.
         replace ((hds ++ [v]) ++ x :: x2) with (hds ++ v :: x :: x2) in H9.
         exact H9.
         rewrite <- app_assoc. auto.
+      + auto.
+      + now inversion PP.
+    - congruence.
+    - now inversion PP.
 Qed.
 
-Theorem term_eval_empty : forall x Fs e, | Fs, e | x ↓ ->
-  exists v k, is_value v /\ ⟨ [], e ⟩ -[k]-> ⟨ [], v ⟩ (* /\ k <= x *).
+Theorem term_eval_empty : forall x Fs e (P : EXPCLOSED e), | Fs, e | x ↓ ->
+  exists v k, VALCLOSED v /\ ⟨ [], e ⟩ -[k]-> ⟨ [], v ⟩ (* /\ k <= x *).
 Proof.
   induction x using lt_wf_ind. destruct x; intros; inversion H0; subst; try congruence.
   * exists e, 0. now repeat constructor.
@@ -1007,9 +997,13 @@ Proof.
   * exists e, 0. split; [ auto | now constructor].
   * apply H in H4. destruct H4, H1, H1. exists x0, (S x1).
     split; [ auto | ]. econstructor. constructor. auto. lia.
+    inversion P. 2: inversion_is_value. apply -> subst_preserves_scope_exp; eauto.
+    apply cons_scope; auto. constructor; auto.
   * exists e, 0. split; [ auto | now constructor ].
-  * exists (EFun [] e0), 0. split; [ constructor | do 2 constructor].
+  * exists (EFun [] e0), 0. inversion P. split; [ auto | do 2 constructor].
   * exists e, 0. split; [ auto | now constructor].
+  * exists e, 0. split; [ auto | now constructor ].
+  * exists e, 0. split; [ auto | now constructor ].
   * exists e, 0. split; [ auto | now constructor ].
   * apply H in H4 as HH. destruct HH, H1, H1. 2: lia.
     eapply frame_indep_nil in H2 as H2_1.
@@ -1019,12 +1013,14 @@ Proof.
       exists x0, (S (x1 + S x2)). split. auto.
       econstructor. constructor. eapply transitive_eval; eauto.
       eapply frame_indep_nil in H2. exact H2.
-      econstructor. constructor. auto.
+      econstructor. constructor. auto. now inversion P.
     - apply H in H11. 2: lia. destruct H11, H3, H3.
       exists x2, (S (x1 + S x3)). split. auto.
       econstructor. constructor. eapply transitive_eval; eauto.
       eapply frame_indep_nil in H2. exact H2.
-      econstructor. constructor; auto. auto.
+      econstructor. constructor; auto. auto. now inversion P.
+    - congruence.
+    - now inversion P.
   * apply H in H4 as HH. destruct HH, H1, H1. 2: lia.
     eapply frame_indep_nil in H2 as H2_1.
     eapply (terminates_step_any_2 _ _ _ _ H4) in H2_1 as H2'.
@@ -1040,6 +1036,11 @@ Proof.
     econstructor. constructor; auto. eapply transitive_eval; eauto.
     eapply frame_indep_nil in H5. exact H5.
     econstructor. constructor. constructor.
+    
+    congruence.
+    now inversion P.
+    congruence.
+    now inversion P.
   * apply H in H4 as v_eval. 2: lia. destruct v_eval, H1, H1.
     eapply frame_indep_nil in H2 as H2_1.
     eapply (terminates_step_any_2 _ _ _ _ H4) in H2_1 as H2'.
@@ -1050,12 +1051,14 @@ Proof.
       econstructor. constructor. eapply transitive_eval; eauto.
       eapply frame_indep_nil in H2. exact H2.
       econstructor. constructor. auto.
+      inversion H1. apply -> subst_preserves_scope_exp; eauto.
+      congruence.
     - inversion H2'; subst; try inversion_is_value.
       
       assert (| FApp2 x0 vs [] :: Fs, e | k ↓) as PP by auto.
       eapply H in H10. 2: lia. destruct H10, H3, H3.
-      destruct (length vs) eqn:P.
-      + apply length_zero_iff_nil in P. subst.
+      destruct (length vs) eqn:P0.
+      + apply length_zero_iff_nil in P0. subst.
         eapply frame_indep_nil in H5 as H5_1.
         eapply (terminates_step_any_2 _ _ _ _ PP) in H5_1 as H5'.
         inversion H5'; subst; try inversion_is_value.
@@ -1064,7 +1067,7 @@ Proof.
         { repeat econstructor; auto. }
         eapply frame_indep_nil in H7.
         epose proof (transitive_eval _ _ _ _ _ H10 _ _ _ H7).
-        assert (⟨ [FApp1 [e]], EFun vl e1 ⟩ -[1]-> ⟨ [FApp2 (EFun vl e1) [] []], e ⟩). { repeat econstructor. }
+        assert (⟨ [FApp1 [e]], EFun vl e1 ⟩ -[1]-> ⟨ [FApp2 (EFun vl e1) [] []], e ⟩). { do 2 econstructor; auto. }
         eapply frame_indep_nil in H2.
         epose proof (transitive_eval _ _ _ _ _ H2 _ _ _ H16).
         eapply frame_indep_nil in H5.
@@ -1073,16 +1076,18 @@ Proof.
         epose proof (transitive_eval _ _ _ _ _ H19 _ _ _ H7).
         exists x0, (S (x1 + 1 + (x3 + 1) + x4)). split; auto.
         econstructor. constructor. auto.
-      + apply eq_sym, last_element_exists in P. destruct P, H6. subst.
+        inversion H1. 2: congruence.
+        apply -> subst_preserves_scope_exp; eauto; subst.
+        simpl. apply cons_scope; auto. rewrite H14. apply cons_scope; auto.
+      + apply eq_sym, last_element_exists in P0. destruct P0, H6. subst.
         eapply frame_indep_nil in H5 as H5_1.
         eapply (terminates_step_any_2 _ _ _ _ PP) in H5_1 as H5'.
-        inversion H8.
         
-        apply app_term_fun_final in H5'; auto.
-        destruct H5', H7, H7. subst. congruence.
+        apply app_term_fun_final in H5' as H5''; auto.
+        destruct H5'' as [vl [e1 [EQ EQ2]]]. subst.
         
         subst.
-        epose proof (eval_app_partial_core_emtpy x4 [] vl e1 x5 _ _ _ _ _ H5' H3 ltac:(auto)).
+        epose proof (eval_app_partial_core_emtpy x4 [] vl e1 x5 _ _ _ _ _ _ _ H5' H3 ltac:(auto)).
         destruct H6, H6, H6, H7. simpl in H10.
         eapply frame_indep_core in H10 as H10_1. simpl in H10_1.
         eapply (terminates_step_any_2 _ _ _ _ H5') in H10_1 as H7'.
@@ -1102,7 +1107,7 @@ Proof.
         epose proof (transitive_eval _ _ _ _ _ H5 _ _ _ H22).
         assert (⟨ [FApp1 (e :: x4 ++ [x5])], EFun vl e1 ⟩ -[1]->
             ⟨ [FApp2 (EFun vl e1) (x4 ++ [x5]) []] , e ⟩).
-            { econstructor. constructor. constructor. constructor. }
+            { econstructor. constructor. auto. constructor. }
         epose proof (transitive_eval _ _ _ _ _ H15 _ _ _ H14).
         eapply frame_indep_nil in H2.
         epose proof (transitive_eval _ _ _ _ _ H2 _ _ _ H16).
@@ -1110,7 +1115,26 @@ Proof.
         exists x9, (S (x1 + (1 + (x3 + (x0 + x8 + 1 + x10))))). split; auto.
         econstructor. constructor. auto.
      Unshelve.
-       all : intros; eapply H. 2: exact H7. all: lia.
+       ** inversion H1. subst. apply -> subst_preserves_scope_exp; eauto.
+          replace (S (Datatypes.length vl) + 0) with (length ((EFun vl e1 :: (x2 :: x6) ++ [x7]))). 2: { simpl. rewrite app_length. simpl in *. lia. }
+          apply scoped_list_idsubst. simpl. do 2 constructor; auto.
+          apply Forall_app; auto.
+        ** congruence.
+        ** inversion P. 2: inversion_is_value.
+           subst. rewrite <- indexed_to_forall in H14.
+           inversion H14. subst. rewrite Forall_app in H16; auto.
+           destruct H16. now inversion H12.
+        ** constructor. auto.
+        ** inversion P. 2: inversion_is_value.
+           rewrite <- indexed_to_forall in H11. now inversion H11.
+        ** constructor. auto.
+        ** inversion P. 2: inversion_is_value.
+           rewrite <- indexed_to_forall in H11. inversion H11.
+           now rewrite Forall_app in H15.
+        ** intros. eapply H. 3: exact H10. lia. auto.
+      + inversion P. 2: inversion_is_value. apply (H7 0); simpl; lia.
+      + congruence.
+    - now inversion P.
   * apply H in H4 as HH. destruct HH, H1, H1. 2: lia.
     eapply frame_indep_nil in H2 as H2_1.
     eapply (terminates_step_any_2 _ _ _ _ H4) in H2_1 as H2'.
@@ -1123,71 +1147,121 @@ Proof.
     econstructor. constructor. eapply transitive_eval; eauto.
     eapply frame_indep_nil in H2. exact H2. 
     econstructor. constructor; auto. auto.
+
+    inversion P. 2: inversion_is_value. 
+    apply -> subst_preserves_scope_exp; eauto.
+    congruence.
+    now inversion P.
+  * apply H in H5 as HH. 2: lia. 2: now inversion P.
+    destruct HH as [v2 [k2 [V2CL Eval2]]].
+    eapply frame_indep_nil in Eval2 as Eval2'.
+    eapply (terminates_step_any_2 _ _ _ _ H5) in Eval2'.
+    inversion Eval2'; subst; try inversion_is_value. 2: congruence.
+    apply H in H8 as [v1 [k1 [V1CL Eval1]]]. 2: lia. 2: now inversion P.
+    assert (⟨ [FCons1 e1], v2 ⟩ -[1]-> ⟨ [FCons2 v2], e1 ⟩).
+    { econstructor. constructor. auto. constructor. }
+    eapply transitive_eval in H1.
+    2: eapply frame_indep_nil in Eval2 as Eval2''; exact Eval2''.
+    eapply frame_indep_nil in Eval1 as Eval1''.
+    eapply transitive_eval in Eval1''. 2: exact H1.
+    assert (⟨ [FCons2 v2], v1 ⟩ -[1]-> ⟨ [], ECons v1 v2 ⟩).
+    { econstructor. constructor; auto. constructor. }
+    eapply transitive_eval in H3. 2: exact Eval1''.
+    exists (ECons v1 v2), (S ((k2 + 1 + k1) + 1)). split. constructor; auto.
+    econstructor. constructor; auto. exact H3.
 Qed.
 
-Corollary term_eval_both : forall x Fs e, | Fs, e | x ↓ ->
-  exists v k, is_value v /\ ⟨ [], e ⟩ -[k]-> ⟨ [], v ⟩ /\ ⟨ Fs, e ⟩ -[k]-> ⟨ Fs, v ⟩.
+Corollary term_eval_both : forall x Fs e (P : EXPCLOSED e), | Fs, e | x ↓ ->
+  exists v k, VALCLOSED v /\ ⟨ [], e ⟩ -[k]-> ⟨ [], v ⟩ /\ ⟨ Fs, e ⟩ -[k]-> ⟨ Fs, v ⟩.
 Proof.
   intros. apply term_eval_empty in H. destruct H, H, H.
   exists x0, x1; split; [| split]; auto.
-  eapply frame_indep_nil in H0; eauto.
+  eapply frame_indep_nil in H0; eauto. auto.
 Qed.
 
-Theorem plus_lit : forall v Fs e x,
+Theorem plus_lit : forall v Fs e x (P: EXPCLOSED e),
   | (FPlus2 v) :: Fs, e | x ↓ -> exists l, v = ELit l.
 Proof.
-  intros. apply term_eval in H as H'. destruct H', H0, H0.
+  intros. apply term_eval in H as H'; auto. destruct H', H0, H0.
   eapply terminates_step_any_2 in H1. 2: exact H.
   inversion H1; subst; try inversion_is_value.
   now exists n.
+  congruence.
 Qed.
 
-Theorem app_term_conditions : forall l1 l2 v e x Fs, 
+Theorem app_term_conditions : forall l1 l2 v e x Fs (P : EXPCLOSED e) (PP : Forall (fun e => EXPCLOSED e) l1), 
   | FApp2 v l1 l2 :: Fs, e | x ↓ ->
-  Forall is_value l2 /\ exists vl e', v = EFun vl e'.
+  Forall (fun v => VALCLOSED v) l2 /\ exists vl e', v = EFun vl e'.
 Proof.
   induction l1; intros.
-  * apply term_eval in H as H'. destruct H', H0, H0.
+  * apply term_eval in H as H'; auto. destruct H', H0, H0.
     eapply (terminates_step_any_2 _ _ _ _ H) in H1 as H1'.
     inversion H1'; subst; try inversion_is_value. split. auto. now do 2 eexists.
+    congruence.
   * apply term_eval in H as H'. destruct H', H0, H0.
     eapply (terminates_step_any_2 _ _ _ _ H) in H1 as H1'.
     inversion H1'; subst; try inversion_is_value. apply IHl1 in H11.
     destruct H11, H3, H3. split; auto. subst. now do 2 eexists.
+    now inversion PP.
+    now inversion PP.
+    congruence.
+    auto.
 Qed.
 
 
 
-Theorem put_back : forall F e Fs,
-  | F :: Fs, e | ↓ -> | Fs, plug_f F e | ↓ /\ frame_wf F.
+Theorem put_back : forall F e Fs (P : EXPCLOSED e) (P2 : FCLOSED F),
+  | F :: Fs, e | ↓ -> | Fs, plug_f F e | ↓.
 Proof.
   destruct F; intros; simpl.
-  * inversion H. split. exists (S x). constructor. auto. constructor.
+  * inversion H. exists (S x). constructor. auto.
   * destruct H.
     apply term_eval in H as H'. destruct H', H0, H0.
     apply app_term_conditions in H as CDS. destruct CDS, H3, H3. subst.
-    split. 2: constructor; auto.
     destruct l2.
-    - simpl in *. exists (2 + x). do 2 constructor.
-      constructor. auto.
+    - simpl in *. exists (2 + x). do 2 constructor; auto.
+      now inversion P2.
     - inversion H2. subst.
-      epose proof (eval_app_partial_core l2 l1 x2 x3 e e0 Fs [] _ H6 H5).
+      epose proof (eval_app_partial_core l2 l1 x2 x3 e e0 Fs [] _ _ H6 H5).
       exists (2 + (S (Datatypes.length l2) + x)). simpl.
-      do 2 constructor. constructor.
+      do 2 constructor. now inversion P2.
       apply terminates_in_k_eq_terminates_in_k_sem in H.
       apply terminates_in_k_eq_terminates_in_k_sem. destruct H, H.
       exists x4. split; auto. rewrite <- Nat.add_succ_l.
       eapply transitive_eval. exact H3. auto.
-  * inversion H. split. exists (S x). constructor. auto. constructor.
-  * inversion H. split. exists (S x). constructor. auto. constructor.
-  * inversion H. apply plus_lit in H0 as H'. destruct H'. subst. split.
-    exists (S (S x)). do 2 constructor. constructor. auto. do 2 constructor.
-  * inversion H. split. exists (S x). constructor. auto. constructor.
+    - auto.
+    - now inversion P2.
+    - auto.
+  * inversion H. exists (S x). constructor. auto.
+  * inversion H. exists (S x). constructor. auto.
+  * inversion H. apply plus_lit in H0 as H'. destruct H'. subst.
+    exists (S (S x)). do 2 constructor. constructor. auto. auto.
+  * inversion H. exists (S x). constructor. auto.
+  * inversion H. inversion P2.
+    (** Shameless trickery: *)
+    apply term_eval in H0 as H0'; subst. destruct H0' as [v2 [k2 [V2CL Eval2]]].
+    assert (⟨ FCons1 e1 :: Fs, e ⟩ -[ k2 + 1 ]-> ⟨ FCons2 v2 :: Fs, e1 ⟩). {
+      eapply transitive_eval; eauto. do 2 econstructor. auto.
+    }
+    eapply terminates_step_any_2 in H1 as H1'. 2: exact H0. 2: auto. inversion P2. subst.
+    apply term_eval in H1' as H1''; subst. destruct H1'' as [v1 [k1 [V1CL Eval1]]].
+    2: auto.
+    assert (⟨ FCons2 v2 :: Fs, e1 ⟩ -[ k1 + 1 ]-> ⟨ Fs, ECons v1 v2 ⟩). {
+      eapply transitive_eval; eauto. do 2 econstructor. auto. auto.
+    }
+    eapply terminates_step_any_2 in H3 as H3'. 2: exact H1'.
+    Search terminates_in_k step_rt.
+    exists (S x). constructor. admit. admit.
+    
+    (* eapply transitive_eval 
+    exists (S x). constructor. auto. *)
+  * inversion H. exists (S x). constructor. admit. admit. (*  auto. *)
 Unshelve.
+  now inversion P2.
   auto.
-Qed.
+Abort.
 
-Theorem put_back_rev : forall F e Fs, frame_wf F ->
+Theorem put_back_rev : forall F e Fs, FCLOSED F ->
   | Fs, plug_f F e | ↓ -> | F :: Fs, e | ↓.
 Proof.
   destruct F; intros; simpl.
@@ -1195,7 +1269,7 @@ Proof.
   * simpl in *. inversion H. subst. destruct H0.
     destruct l2.
     - simpl in H0. inversion H0; subst; try inversion_is_value.
-      inversion H6; subst; try inversion_is_value. eexists. eauto.
+      inversion H8; subst; try inversion_is_value. eexists. eauto.
     - inversion H2. subst. inversion H0; subst; try inversion_is_value.
       inversion H8; subst; try inversion_is_value.
       epose proof (eval_app_partial_core l2 l1 vl b e e0 Fs [] ltac:(auto) H5 H4).
@@ -1208,8 +1282,8 @@ Proof.
   * destruct H0. simpl in H0. inversion H0; subst; try inversion_is_value. eexists. eauto.
 Qed.
 
-Theorem term_app_in_k : forall Fs vl vals e k,
-  length vl = length vals -> Forall is_value vals ->
+Theorem term_app_in_k : forall Fs vl vals e k (P : VALCLOSED (EFun vl e)),
+  length vl = length vals -> Forall (fun v => VALCLOSED v) vals ->
   | Fs, e.[EFun vl e .: list_subst vals idsubst] | k ↓ ->
   | Fs, EApp (EFun vl e) vals | 2 + length vl + k ↓.
 Proof.
@@ -1218,17 +1292,20 @@ Proof.
     do 2 constructor. auto.
   * destruct (length l) eqn:D1.
     - apply length_zero_iff_nil in D1. subst. rewrite H. simpl.
-      do 3 constructor; auto.
+      do 2 constructor; auto. now constructor.
     - apply eq_sym, last_element_exists in D1 as D1'. destruct D1' as [l' [l'x EQ]].
       subst. apply Forall_app in H3 as [H3_1 H3_2]. inversion H3_2. subst.
       epose proof (eval_app_partial_core l' [] vl e l'x x Fs []
-         ltac:(constructor) H3_1 H2). cbn in H3.
+         ltac:(constructor) _ H3_1 H2). cbn in H3.
       assert (⟨ FApp2 (EFun vl e) [] (x :: l') :: Fs, l'x ⟩ -[1]-> ⟨ Fs, e.[EFun vl e .: list_subst (x :: l' ++ [l'x]) idsubst] ⟩). { 
         econstructor; constructor. all: auto.
         simpl. simpl in H. rewrite app_length in H. simpl in H. lia.
       }
       epose proof (transitive_eval _ _ _ _ _ H3 _ _ _ H4).
       eapply term_step_term_plus in H7. 2: exact H1.
-      rewrite H. simpl. rewrite app_length. simpl. repeat constructor. exact H7.
+      rewrite H. simpl. rewrite app_length. simpl. do 2 constructor. auto. exact H7.
+  Unshelve.
+    now inversion P.
+    auto.
 Qed.
 
